siftDown lemma passes

Heapsort.fst
@@ -26,12 +26,8 @@ let rec all p h =
   | Leaf -> true
   | Node n h1 h2 -> p n && all p h1 && all p h2
 
-val lt : nat -> nat -> Tot bool
-let lt n1 n2 = n1 < n2
-
-val gt : nat -> nat -> Tot bool
-let gt n1 n2 = n1 > n2
-
+val lte : nat -> nat -> Tot bool
+let lte n1 n2 = n1 <= n2
 
 val is_heap : heap -> (nat -> nat -> Tot bool) -> Tot bool
 let rec is_heap h c =
@@ -40,7 +36,26 @@ let rec is_heap h c =
   | Node n h1 h2 -> all (c n) h1 && all (c n) h2 && is_heap h1 c && is_heap h2 c
   
 val is_minHeap : heap -> Tot bool
-let rec is_minHeap h = is_heap h lt
+let rec is_minHeap h = is_heap h lte
+
+
+val heapLeft: h:heap{is_minHeap h} -> l:heap{is_minHeap l}
+let heapLeft h =
+  match h with 
+  | Leaf -> Leaf
+  | Node m l r -> l
+
+val heapRight: h:heap{is_minHeap h} -> r:heap{is_minHeap r}
+let heapRight h =
+  match h with 
+  | Leaf -> Leaf
+  | Node m l r -> r
+
+val heapVal: h:heap{is_minHeap h} -> n:nat
+let heapVal h =
+  match h with 
+  | Leaf -> 0
+  | Node m l r -> m
 
 val insertMinHeap : n:nat -> h:heap{is_minHeap h} -> 
     Tot (o:heap{is_minHeap o /\ (forall m. in_heap m o <==> (in_heap m h \/ m = n))}) (decreases h)
@@ -51,20 +66,49 @@ let rec insertMinHeap n h =
                     (if m < n then Node m (insertMinHeap n h2) h1 
                     else Node n (insertMinHeap m h2) h1)
 
-val siftDown: n:nat -> l:heap -> r:heap -> Tot (o:heap) (decreases ((size l)+(size r)))
+(* doesn't work*)
+(**)
+(*val siftDown: n:nat -> l:heap{is_minHeap l /\ ~(in_heap n l)} -> r:heap{is_minHeap r /\ ~(in_heap n r)}  -> 
+    Tot (o:heap{is_minHeap o}) (decreases ((size l)+(size r)))*)
+//val siftDown: n:nat -> l:heap -> r:heap  -> Tot (o:heap) (decreases ((size l)+(size r)))
+val siftDown: n:nat -> l:heap{is_minHeap l} -> r:heap{is_minHeap r}  -> Tot (o:heap{is_minHeap o}) (decreases ((size l)+(size r)))
 let rec siftDown n l r = 
   match l with 
   | Leaf -> Node n Leaf Leaf
   | Node m1 m1l m1r ->
     match r with
     | Leaf -> 
-        if n < m1 then (Node n l Leaf)
+        if n <= m1 then (Node n l Leaf)
         else (Node m1 (Node n Leaf Leaf) Leaf)
     | Node m2 m2l m2r -> 
-        if n < m1 && n < m2 then Node n l r
-        else if m1 < m2 then Node m1 (siftDown n m1l m1r) r
-        else  Node m2 l (siftDown n m2l m2r)
+        if n <= m1 && n <= m2 then Node n l r
+        else if m1 <= n && m1 <= m2 then (Node m1 (siftDown n m1l m1r) r)
+        else (Node m2 l (siftDown n m2l m2r) )
+///////
+val siftDown_lemma: n:nat -> l:heap{is_minHeap l} -> r:heap{is_minHeap r}  -> 
+    Lemma (ensures
+      ((heapVal l = 0) ==> is_minHeap (Node n Leaf Leaf))
+      \/ ( ~(heapVal l = 0) /\ (heapVal r = 0) /\ n  <= (heapVal l)  ==> is_minHeap (Node n l Leaf))
+      \/ ( ~(heapVal l = 0) /\ (heapVal r = 0) /\  n > (heapVal l)  ==> is_minHeap (Node (heapVal l) (Node n Leaf Leaf) Leaf) )
+      \/ (~(heapVal r = 0) /\ ~(heapVal l = 0) /\ (heapVal l) > n /\ (heapVal r) > n ==> is_minHeap (Node n l r))
+      \/ (~(heapVal r = 0) /\ ~(heapVal l = 0) /\ (heapVal l) <= n /\ (heapVal l) <= (heapVal r) ==> is_minHeap (Node (heapVal l) (siftDown n (heapLeft l) (heapRight l)) r) )
+      \/ (~(heapVal r = 0) /\ ~(heapVal l = 0) /\ (heapVal r) < n /\ (heapVal r) < (heapVal l) ==> is_minHeap (Node (heapVal r) l (siftDown n (heapLeft r) (heapRight r) ) ) )
+      ) [SMTPat (siftDown n l r)]
+let rec siftDown_lemma n l r = 
+  match l with 
+  | Leaf -> ()
+  | Node m1 m1l m1r ->
+    match r with
+    | Leaf -> 
+        if n <= m1 then ()
+        else ()
+    | Node m2 m2l m2r -> 
+        if n <= m1 && n <= m2 then (assert(is_minHeap (Node n l r))) 
+        else if m1 <= n && m1 <= m2 then (assert(is_minHeap m1r); assert(is_minHeap m1l); (siftDown_lemma m1 (siftDown n m1l m1r) r) )
+        else (assert(is_minHeap m2r); assert(is_minHeap m2l);  (siftDown_lemma m2 l (siftDown n m2l m2r)) )
 
+(*
+val leftRem: h:heap{is_minHeap h} -> Tot (n:nat * o:heap{is_minHeap o})*)
 val leftRem: h:heap -> Tot (n:nat * o:heap)
 let rec leftRem h = 
     match h with
@@ -74,7 +118,7 @@ let rec leftRem h =
           match (leftRem l) with
           | (m1, l2) -> (m1, Node m r l2)
 
-
+(*val deleteMin: h:heap{is_minHeap h} -> Tot (o:heap{is_minHeap h})*)
 val deleteMin: h:heap -> Tot (o:heap)
 let deleteMin h = 
         match h with
@@ -94,16 +138,19 @@ let peek h =
   match h with 
   | Leaf -> 0
   | Node n _ _ -> n
-  
 
-val printAndDelete: h:heap -> ML unit
+(*val printAndDelete: h:heap -> ML unit*)
+val printAndDelete: h:heap{is_minHeap h} -> ML unit
 let rec printAndDelete h =
   match h with 
   | Leaf -> ()
   | Node _ _ _ ->
   let v1 = peek h in
-  FStar.IO.print_string ("Min" ^ string_of_int(v1) ^ "\n"); 
-  printAndDelete(deleteMin h) 
+  FStar.IO.print_string ("Min " ^ string_of_int(v1) ^ "\n"); 
+  match (deleteMin h) with 
+  | Leaf -> ()
+  | Node x Leaf Leaf ->  FStar.IO.print_string ("Min " ^ string_of_int(x) ^ "\n")
+  | Node _ _ _ ->  printAndDelete( (deleteMin h) ) 
 
 val checking : unit -> ML unit
 let checking () =
@@ -112,8 +159,12 @@ let checking () =
   let h3 = insertMinHeap 9 h2 in 
   let h4 = insertMinHeap 7 h3 in 
   let h5 = insertMinHeap 2 h4 in 
-  let h6 = insertMinHeap 4 h5 in 
-  printAndDelete h6
+  let h6 = insertMinHeap 1 h5 in 
+  let h7 = insertMinHeap 4 h6 in 
+  let h8 = insertMinHeap 10 h7 in 
+  let h9 = insertMinHeap 6 h8 in 
+  let h10 = insertMinHeap 8 h9 in 
+  printAndDelete h10
   (*
   FStar.IO.print_string ("Min" ^ string_of_int(peekMin h6) ^ "\n");
   let h7 = deleteMin h6 in
@@ -123,5 +174,4 @@ let checking () =
   let h9 = deleteMin h8 in
   FStar.IO.print_string ("Min" ^ string_of_int(peekMin h9) ^ "\n")
 *)
-
 let main = checking()
